src/Rupicola/Examples/Uppercase.v
@@ -31,7 +31,7 @@ Require Import bedrock2.BasicC32Semantics.
 Section Impl.
   Definition upchar_impl (b: byte) :=
     if word.wrap (byte.unsigned b - byte.unsigned "a"%byte) <? 26
-    then byte_land b x5f else b.
+    then byte.and b x5f else b.
 
   Lemma upchar_impl_ok b:
     upchar_spec b = upchar_impl b.
